Johannes's ffi_state_cor definition

projection/proofs/to_cake/payload_to_cakemlProofScript.sml
@@ -1742,10 +1742,10 @@ QED
 (* -- Check identifier and FFI model contains
       correct messages *)
 Definition ffi_state_cor_def:
-  ffi_state_cor cpNum pSt (fNum,fQueue,fNet) ⇔
+  ffi_state_cor conf cpNum pSt (fNum,fQueue,fNet) ⇔
     cpNum = fNum ∧
-    ∀sp.
-      isPREFIX (qlk pSt.queues sp) (qlk fQueue sp)
+    ∃fNet1.
+      ffi_eq conf (fNum,fQueue,fNet) (fNum,pSt.queues,fNet1)
 End
 
 (* Combined *)
@@ -1756,7 +1756,7 @@ Definition cpEval_valid_def:
     enc_ok conf cEnv (letfuns pCd) vs ∧
     pSt_pCd_corr pSt pCd ∧
     sem_env_cor conf pSt cEnv ∧
-    ffi_state_cor cpNum pSt cSt.ffi.ffi_state ∧
+    ffi_state_cor conf cpNum pSt cSt.ffi.ffi_state ∧
     ffi_wf cSt.ffi.ffi_state ∧
     cSt.ffi.oracle = comms_ffi_oracle conf
 End
@@ -1935,36 +1935,51 @@ Proof
                   MAP_EVERY qexists_tac [‘P’,‘l’] >> rw[]) >>
   metis_tac[send_events_is_stream]
 QED
+
+Theorem ffi_eq_bisimulation_L:
+  ffi_eq conf s1 s2 ∧ strans conf s1 L s1' ⇒
+  ∃s2'. ffi_eq conf s1' s2' ∧ strans conf s2 L s2'
+Proof
+  simp[ffi_eq_def] >>
+  simp[SimpL “$==>”, Once bisimulationTheory.BISIM_REL_cases] >>
+  metis_tac[]
+QED
+
+
+
 (* A stream of valid send events cannot break FFI correspondence*)
 Theorem ffi_state_cor_send_stream_irrel:
   ∀conf cpNum pSt ckFSt l send_stream P.
-    ffi_state_cor cpNum pSt ckFSt ∧
+    ffi_state_cor conf cpNum pSt ckFSt ∧
     EVERY (valid_send_event_format conf l) send_stream ∧
     ffi_accepts_rel P (valid_send_call_format conf l) (comms_ffi_oracle conf) ∧
     P ckFSt
     ⇒
-    ffi_state_cor cpNum pSt (update_state ckFSt (comms_ffi_oracle conf) send_stream)
+    ffi_state_cor conf cpNum pSt
+      (update_state ckFSt (comms_ffi_oracle conf) send_stream)
 Proof
   Induct_on ‘send_stream’ >>
   rw[update_state_def] >>
   Cases_on ‘h’ >>
   PURE_ONCE_REWRITE_TAC [update_state_def] >>
-  qmatch_goalsub_abbrev_tac ‘ffi_state_cor cpNum pSt (update_state ckFSt1 _ send_stream)’ >>
+  qmatch_goalsub_abbrev_tac
+    ‘ffi_state_cor conf cpNum pSt (update_state ckFSt1 _ send_stream)’ >>
   rename1 ‘valid_send_event_format conf l (IO_event s l' d)’ >>
   ‘l' = l’
     by fs[valid_send_event_format_def,valid_send_call_format_def] >>
   fs[] >>
   first_x_assum (K ALL_TAC) >>
   last_x_assum irule >>
-  qpat_assum ‘ffi_accepts_rel _ _ _’ (assume_tac o (REWRITE_RULE [ffi_accepts_rel_def])) >>
+  qpat_assum ‘ffi_accepts_rel _ _ _’
+             (assume_tac o (REWRITE_RULE [ffi_accepts_rel_def])) >>
   first_x_assum (qspecl_then [‘<|oracle := comms_ffi_oracle conf;
-                               ffi_state := ckFSt;
-                               io_events := ARB|>’,
-                               ‘s’,‘l’,‘MAP FST d’]
+                                 ffi_state := ckFSt;
+                                 io_events := ARB|>’,
+                              ‘s’,‘l’,‘MAP FST d’]
                            strip_assume_tac) >>
   rfs[valid_send_event_format_def] >>
   fs[] >> qunabbrev_tac ‘ckFSt1’ >>
-  qmatch_goalsub_rename_tac ‘ffi_state_cor _ _ ckFSt1’ >>
+  qmatch_goalsub_rename_tac ‘ffi_state_cor _ _ _ ckFSt1’ >>
   rw[]
   >- (MAP_EVERY qexists_tac [‘P’,‘l’] >> fs[]) >>
   fs[ffi_accepts_rel_def,valid_send_event_format_def] >>
@@ -1974,26 +1989,24 @@ Proof
   ‘s = "send"’
     by fs[valid_send_call_format_def] >>
   fs[ffi_send_def] >> first_x_assum (K ALL_TAC) >>
-  Cases_on ‘∃ns. strans conf ckFSt (ASend l (MAP SND d)) ns’ >>
-  Cases_on ‘LENGTH d = SUC conf.payload_size’ >>
-  fs[some_def] >> rw[] >>
+  fs[AllCaseEqs(), some_def] >>
+  rw[] >>
   irule SELECT_ELIM_THM >>
   rw[]
   >- (qpat_x_assum ‘strans _ _ _ ns’ (K ALL_TAC) >>
-      qmatch_goalsub_rename_tac ‘ffi_state_cor _  _ ns’ >>
+      qmatch_goalsub_rename_tac ‘ffi_state_cor _ _ _ ns’ >>
       Cases_on ‘ns’ >> Cases_on ‘ckFSt’ >>
       rename1 ‘strans conf (PN,R) _ (PN',R')’ >>
-      ‘PN' = PN’
-        by (drule strans_pres_pnum >>
-            simp[]) >>
+      ‘PN' = PN’ by (drule strans_pres_pnum >> simp[]) >>
       fs[] >> first_x_assum (K ALL_TAC) >>
       ‘PN = cpNum’
-        by (Cases_on ‘R’ >>
-            fs[ffi_state_cor_def]) >>
-      fs[] >>
-      first_x_assum (K ALL_TAC) >>
+        by (Cases_on ‘R’ >> fs[ffi_state_cor_def]) >>
+      pop_assum SUBST_ALL_TAC
       Cases_on ‘R’ >> Cases_on ‘R'’ >>
       rename1 ‘strans conf (_,Q,N) _ (_,Q',N')’ >>
+      fs[ffi_state_cor_def] >>
+      metis_tac[ffi_eq_bisimulation_L]
+
       ‘∀sp.
         isPREFIX (qlk Q sp) (qlk Q' sp)’
         suffices_by (rw[] >> fs[ffi_state_cor_def] >>
@@ -2799,6 +2812,7 @@ Proof
   fs[valid_send_dest_def]
 QED
 
+
 (* FORWARD CORRECTNESS
     Just the spec :) *)
 Theorem endpoint_forward_correctness:
@@ -3044,6 +3058,12 @@ Proof
           simp[] >> fs[cpEval_valid_def]) >>
       disch_then (qx_choose_then ‘MC’ assume_tac) >>
       qexists_tac ‘MC’ >> dxrule cEval_equiv_bump_clocks >> simp[])
+  >- ((* LReceive case *)
+      CONV_TAC SWAP_VARS_CONV >> qexists_tac ‘vs1’ >>
+      CONV_TAC SWAP_VARS_CONV >> qexists_tac ‘cEnv1’ >>
+      simp[GSYM PULL_EXISTS] >> conj_tac
+      >- (fs[cpEval_valid_def, pSt_pCd_corr_def, sem_env_cor_def] >> conj_tac
+          >- (fs[ffi_state_cor_def, cpFFI_valid_def]
   >> cheat
 QED
 
